{
 "cells": [
  {
   "cell_type": "markdown",
   "id": "63633895-6308-40a9-b738-e3e81dfa5594",
   "metadata": {},
   "source": [
    "# Logistic ODE to Logistic Map\n",
    "\n",
    "$$ p_{n+1} = p_n + kp_n(1-\\frac{p_n}{C}) $$\n",
    "\n",
    "Multiply everything by C\n",
    "\n",
    "$$ C*p_{n+1} = C*p_n + C*kp_n(1-\\frac{p_n}{C}) $$\n",
    "\n",
    "Let $x_n = \\frac{p_n}{C}$ and plug it in to give us:\n",
    "\n",
    "$$ x_{n+1} = x_n + kx_n(1-x_n) $$\n",
    "\n",
    "Factor out $x_n$\n",
    "\n",
    "$$ x_{n+1} = x_n(1 + k - kx_n)$$\n",
    "\n",
    "$$x_{n+1} = -kx_n^2 + (1+k)x_n $$\n",
    "\n",
    "Multiply everything by $\\frac{k}{k+1}$\n",
    "\n",
    "$$\\frac{k}{k+1}x_{n+1} = \\frac{k}{k+1}(-kx_n^2 + (1+k)x_n) $$\n",
    "\n",
    "$$\\frac{k}{k+1}x_{n+1} = -\\frac{k^2}{k+1}x_n^2 + kx_n $$\n",
    "\n",
    "Now if we let $l_n = \\frac{k+1}{k}x_n$ then we can plug that in and get\n",
    "\n",
    "$$l_{n+1} = -(k+1)l_n^2 + (k+1)l_n $$\n",
    "\n",
    "$$l_{n+1} = (k+1)l_n(-l_n + 1) $$\n",
    "\n",
    "$$l_{n+1} = (k+1)l_n(1 - l_n) $$\n",
    "\n",
    "Let r = k+1 and we end up with the logistic map!\n",
    "\n",
    "$$l_{n+1} = rl_n(1-l_n) $$"
   ]
  },
  {
   "cell_type": "code",
   "execution_count": null,
   "id": "628a85c0-e270-4311-99a3-e6d414e7e381",
   "metadata": {},
   "outputs": [],
   "source": []
  }
 ],
 "metadata": {
  "kernelspec": {
   "display_name": "Python 3 (ipykernel)",
   "language": "python",
   "name": "python3"
  },
  "language_info": {
   "codemirror_mode": {
    "name": "ipython",
    "version": 3
   },
   "file_extension": ".py",
   "mimetype": "text/x-python",
   "name": "python",
   "nbconvert_exporter": "python",
   "pygments_lexer": "ipython3",
   "version": "3.12.7"
  }
 },
 "nbformat": 4,
 "nbformat_minor": 5
}
